Semantics.thy
@@ -33,7 +33,8 @@ locale semantics =
 
 locale semantics =
   fixes exists_act :: "'a"
-  fixes exists_state :: "'b::state"
+  fixes exists_state :: "'b::pstate"
+  fixes exists_aux :: "'c"
 
 
 context semantics
