SimAsm/SimAsm.thy
@@ -68,12 +68,15 @@ definition liftl :: "('v,'g,'r) op \<Rightarrow> ('v,'g,'r,'a) opbasic"
 
 section \<open>Language Definition\<close>
 
+
+(* predicates are no longer sets of states but sets of trees, ie., of type predTree *)
+
 datatype ('v,'g,'r,'a) lang =
   Skip
-  | Op "('v,'g,'r,'a) pred" "('v,'g,'r) op" "('v,'g,'r,'a) auxfn"
+  | Op "('v,'g,'r,'a) predTree" "('v,'g,'r) op" "('v,'g,'r,'a) auxfn"
   | Seq "('v,'g,'r,'a) lang" "('v,'g,'r,'a) lang"
   | If "('v,'g,'r) bexp" "('v,'g,'r,'a) lang" "('v,'g,'r,'a) lang"
-  | While "('v,'g,'r) bexp" "('v,'g,'r,'a) pred" "('v,'g,'r,'a) lang"
-  | DoWhile "('v,'g,'r,'a) pred" "('v,'g,'r,'a) lang" "('v,'g,'r) bexp"
+  | While "('v,'g,'r) bexp" "('v,'g,'r,'a) predTree" "('v,'g,'r,'a) lang"
+  | DoWhile "('v,'g,'r,'a) predTree" "('v,'g,'r,'a) lang" "('v,'g,'r) bexp"
 
 end
